bunch of progress

cedar-lean/Cedar/Spec/Evaluator.lean
@@ -77,49 +77,43 @@ def bindAttr (a : Attr) (res : Result Value) : Result (Attr × Value) := do
   let v ← res
   ok (a, v)
 
-class ConcreteEvaluatable (α : Type) where
-  eval : (a : α) -> (req : Request) -> (es : Entities) -> Result Value
-
-instance [ConcreteEvaluatable α] : ConcreteEvaluatable (Expr α) where
-  eval (x : Expr α) req es :=
+def evaluate (x : Expr) (req : Request) (es : Entities) : Result Value :=
   match x with
-  | .lit l       => ok l
-  | .var var     =>
-    match var with
-    | .principal => ok req.principal
-    | .action    => ok req.action
-    | .resource  => ok req.resource
-    | .context   => ok req.context
-  | .ite x₁ x₂ x₃ => do
-    let b ← (ConcreteEvaluatable.eval x₁ req es).as Bool
-    if b then ConcreteEvaluatable.eval x₂ req es else ConcreteEvaluatable.eval x₃ req es
-  | .and x₁ x₂   => do
-    let b ← (ConcreteEvaluatable.eval x₁ req es).as Bool
-    if !b then ok b else (ConcreteEvaluatable.eval x₂ req es).as Bool
-  | .or x₁ x₂    => do
-    let b ← (ConcreteEvaluatable.eval x₁ req es).as Bool
-    if b then ok b else (ConcreteEvaluatable.eval x₂ req es).as Bool
-  | .unaryApp op₁ x₁     => do
-    let v₁ ← ConcreteEvaluatable.eval x₁ req es
+  | .lit l          => ok l
+  | .var .principal => ok req.principal
+  | .var .action    => ok req.action
+  | .var .resource  => ok req.resource
+  | .var .context   => ok req.context
+  | .ite x₁ x₂ x₃   => do
+    let b ← (evaluate x₁ req es).as Bool
+    if b then evaluate x₂ req es else evaluate x₃ req es
+  | .and x₁ x₂      => do
+    let b ← (evaluate x₁ req es).as Bool
+    if !b then ok b else (evaluate x₂ req es).as Bool
+  | .or x₁ x₂       => do
+    let b ← (evaluate x₁ req es).as Bool
+    if b then ok b else (evaluate x₂ req es).as Bool
+  | .unaryApp op₁ x₁ => do
+    let v₁ ← evaluate x₁ req es
     apply₁ op₁ v₁
   | .binaryApp op₂ x₁ x₂ => do
-    let v₁ ← ConcreteEvaluatable.eval x₁ req es
-    let v₂ ← ConcreteEvaluatable.eval x₂ req es
+    let v₁ ← evaluate x₁ req es
+    let v₂ ← evaluate x₂ req es
     apply₂ op₂ v₁ v₂ es
-  | .hasAttr x₁ a        => do
-    let v₁ ← ConcreteEvaluatable.eval x₁ req es
+  | .hasAttr x₁ a   => do
+    let v₁ ← evaluate x₁ req es
     hasAttr v₁ a es
-  | .getAttr x₁ a        => do
-    let v₁ ← ConcreteEvaluatable.eval x₁ req es
+  | .getAttr x₁ a   => do
+    let v₁ ← evaluate x₁ req es
     getAttr v₁ a es
-  | .set xs              => do
-    let vs ← xs.mapM₁ (fun ⟨x₁, _⟩ => ConcreteEvaluatable.eval x₁ req es)
+  | .set xs         => do
+    let vs ← xs.mapM₁ (fun ⟨x₁, _⟩ => evaluate x₁ req es)
     ok (Set.make vs)
-  | .record axs          => do
-    let avs ← axs.mapM₂ (fun ⟨(a₁, x₁), _⟩ => bindAttr a₁ (ConcreteEvaluatable.eval x₁ req es))
+  | .record axs     => do
+    let avs ← axs.mapM₂ (fun ⟨(a₁, x₁), _⟩ => bindAttr a₁ (evaluate x₁ req es))
     ok (Map.make avs)
-  | .call xfn xs         => do
-    let vs ← xs.mapM₁ (fun ⟨x₁, _⟩ => ConcreteEvaluatable.eval x₁ req es)
+  | .call xfn xs    => do
+    let vs ← xs.mapM₁ (fun ⟨x₁, _⟩ => evaluate x₁ req es)
     call xfn vs
 
 end Cedar.Spec
