cedar-lean/Cedar/Spec/PartialEvaluator.lean
@@ -14,77 +14,144 @@
  limitations under the License.
 -/
 
-import Cedar.Spec.Entities
 import Cedar.Spec.Evaluator
-import Cedar.Spec.Expr
-import Cedar.Spec.Request
+import Cedar.Spec.PartialEntities
+import Cedar.Spec.PartialExpr
+import Cedar.Spec.PartialRequest
+import Cedar.Spec.PartialValue
+import Cedar.Spec.Value
 
 /-! This file defines the semantics of Cedar partial evaluation. -/
 
 namespace Cedar.Spec
 
 open Cedar.Data
+open Except
+open Error
 
-/--
-  Identical to `Expr` except that it has an `unknown` case, and the recursive
-  elements are also all `PartialExpr` instead of `Expr`
--/
-inductive PartialExpr where
-  | expr (expr : Expr PartialExpr)
-  | unknown
+def partialInₑ (uid₁ uid₂ : EntityUID) (es : PartialEntities) : Bool :=
+  uid₁ == uid₂ || (es.ancestorsOrEmpty uid₁).contains uid₂
 
-inductive PartialValue where
-  | value (v : Value)
-  | residual (r : PartialExpr)
+def partialInₛ (uid : EntityUID) (vs : Set Value) (es : PartialEntities) : Result Value := do
+  let uids ← vs.mapOrErr Value.asEntityUID .typeError
+  ok (uids.any (partialInₑ uid · es))
 
-inductive PartialRequest where
-  | known (req : Request)
+def partialApply₂ (op₂ : BinaryOp) (v₁ v₂ : Value) (es : PartialEntities) : Result PartialValue :=
+  match op₂, v₁, v₂ with
+  | .eq, _, _                                              => ok (.value (v₁ == v₂))
+  | .less,   .prim (.int i), .prim (.int j)                => ok (.value ((i < j): Bool))
+  | .lessEq, .prim (.int i), .prim (.int j)                => ok (.value ((i ≤ j): Bool))
+  | .add,    .prim (.int i), .prim (.int j)                => intOrErr (i.add? j) >>= fun x => ok (.value x)
+  | .sub,    .prim (.int i), .prim (.int j)                => intOrErr (i.sub? j) >>= fun x => ok (.value x)
+  | .contains,    .set vs₁, _                              => ok (.value (vs₁.contains v₂))
+  | .containsAll, .set vs₁, .set vs₂                       => ok (.value (vs₂.subset vs₁))
+  | .containsAny, .set vs₁, .set vs₂                       => ok (.value (vs₁.intersects vs₂))
+  | .mem, .prim (.entityUID uid₁), .prim (.entityUID uid₂) => ok (.value (partialInₑ uid₁ uid₂ es))
+  | .mem, .prim (.entityUID uid₁), .set (vs)               => partialInₛ uid₁ vs es >>= fun x => ok (.value x)
+  | _, _, _                                                => error .typeError
 
-inductive PartialEntities where
-  | known (entities : Entities)
+def partialAttrsOf (v : Value) (lookup : EntityUID → Result (Map Attr PartialValue)) : Result (Map Attr PartialValue) :=
+  match v with
+  | .record r              => ok (r.mapOnValues PartialValue.value)
+  | .prim (.entityUID uid) => lookup uid
+  | _                      => error typeError
 
-class PartialEvaluatable (α : Type) where
-  partialEval : (a : α) -> (req : PartialRequest) -> (es : PartialEntities) -> Result PartialValue
+def partialHasAttr (v : Value) (a : Attr) (es : PartialEntities) : Result Value := do
+  let r ← partialAttrsOf v (fun uid => ok (es.attrsOrEmpty uid))
+  ok (r.contains a)
 
-def liftConcrete (res : Result Value) : Result PartialValue :=
-  match res with
-  | .ok val => .ok (.value val)
-  | .error e => .error e
+def partialGetAttr (v : Value) (a : Attr) (es : PartialEntities) : Result PartialValue := do
+  let r ← partialAttrsOf v es.attrs
+  r.findOrErr a attrDoesNotExist
 
-instance [ConcreteEvaluatable α] : PartialEvaluatable α where
-  partialEval (x : α) req es :=
-  match (req, es) with
-  | (.known req, .known es) => liftConcrete (ConcreteEvaluatable.eval x req es)
+def partialBindAttr (a : Attr) (res : Result PartialValue) : Result (Attr × PartialValue) := do
+  let v ← res
+  ok (a, v)
 
-mutual
-
-instance [PartialEvaluatable α] : PartialEvaluatable (Expr α) where
-  partialEval (x : Expr α) req es :=
-  match (req, es) with
-  | (.known known_req, .known known_es) =>
-    match x with
-    | .lit l => liftConcrete (ConcreteEvaluatable.eval (Expr.lit l) known_req known_es)
-    | .var v => liftConcrete (ConcreteEvaluatable.eval (Expr.var v) known_req known_es)
-    /-
-    | .ite x₁ x₂ x₃ => do
-      let b ← (PartialEvaluatable.partialEval x₁ req es)
-      match b with
-      | .value v => do
-        let b ← b.as Bool
-        if b then PartialEvaluatable.partialEval x₂ req es else PartialEvaluatable.partialEval x₃ req es
-    -/
-    | .unaryApp op₁ x₁ => do
-      let pval ← PartialEvaluatable.partialEval x₁ req es
-      match pval with
-        | .value val => do
-          let val ← apply₁ op₁ val -- TODO: reuse the concrete evaluator code somehow
-          .ok (.value val)
-        | .residual r => .ok (.residual (PartialExpr.expr (Expr.unaryApp op₁ r)))
-
-instance : PartialEvaluatable PartialExpr where
-  partialEval (x : PartialExpr) req es :=
+def partialEvaluate (x : PartialExpr) (req : PartialRequest) (es : PartialEntities) : Result PartialValue :=
   match x with
-  | .expr expr => PartialEvaluatable.partialEval expr req es
-  | .unknown => .ok (.residual x)
-
-end
+  | .lit l          => ok (.value l)
+  | .var .principal => ok req.principal
+  | .var .action    => ok req.action
+  | .var .resource  => ok req.resource
+  | .var .context   => match req.context.kvs.mapM fun (k, v) => match v with | .value v => some (k, v) | .residual _ => none with
+    | some kvs      => ok (.value (Map.make kvs))
+    | none          => ok (.residual (PartialExpr.record (req.context.kvs.map fun (k, v) => (k, v.asPartialExpr))))
+  | .ite x₁ x₂ x₃   => do
+    let pval ← partialEvaluate x₁ req es
+    match pval with
+    | .value v => do
+      let b ← v.asBool
+      if b then partialEvaluate x₂ req es else partialEvaluate x₃ req es
+    | .residual r => ok (.residual (PartialExpr.ite r x₂ x₃))
+  | .and x₁ x₂   => do
+    let pval ← partialEvaluate x₁ req es
+    match pval with
+    | .value v => do
+      let b ← v.asBool
+      if !b then ok (.value b) else do
+        let pval ← partialEvaluate x₂ req es
+        match pval with
+        | .value v => do
+          let b ← v.asBool
+          ok (.value b)
+        | .residual r => ok (.residual r)
+    | .residual r => ok (.residual (PartialExpr.and r x₂))
+  | .or x₁ x₂    => do
+    let pval ← partialEvaluate x₁ req es
+    match pval with
+    | .value v => do
+      let b ← v.asBool
+      if b then ok (.value b) else do
+        let pval ← partialEvaluate x₂ req es
+        match pval with
+        | .value v => do
+          let b ← v.asBool
+          ok (.value b)
+        | .residual r => ok (.residual r)
+    | .residual r => ok (.residual (PartialExpr.or r x₂))
+  | .unaryApp op₁ x₁     => do
+    let pval ← partialEvaluate x₁ req es
+    match pval with
+    | .value v₁ => do
+      let val ← apply₁ op₁ v₁
+      ok (.value val)
+    | .residual r => ok (.residual (PartialExpr.unaryApp op₁ r))
+  | .binaryApp op₂ x₁ x₂ => do
+    let pval₁ ← partialEvaluate x₁ req es
+    let pval₂ ← partialEvaluate x₂ req es
+    match (pval₁, pval₂) with
+    | (.value v₁, .value v₂) => partialApply₂ op₂ v₁ v₂ es
+    | (.value v₁, .residual r₂) => ok (.residual (PartialExpr.binaryApp op₂ v₁.asPartialExpr r₂))
+    | (.residual r₁, .value v₂) => ok (.residual (PartialExpr.binaryApp op₂ r₁ v₂.asPartialExpr))
+    | (.residual r₁, .residual r₂) => ok (.residual (PartialExpr.binaryApp op₂ r₁ r₂))
+  | .hasAttr x₁ a        => do
+    let pval₁ ← partialEvaluate x₁ req es
+    match pval₁ with
+    | .value v₁ => do
+      let val ← partialHasAttr v₁ a es
+      ok (.value val)
+    | .residual r => ok (.residual (PartialExpr.hasAttr r a)) -- TODO more precise: even though pval₁ is a residual we may know concretely whether it contains the particular attr we care about
+  | .getAttr x₁ a        => do
+    let pval₁ ← partialEvaluate x₁ req es
+    match pval₁ with
+    | .value v₁ => partialGetAttr v₁ a es
+    | .residual r => ok (.residual (PartialExpr.getAttr r a)) -- TODO more precise: pval₁ will be a .residual if it contains any unknowns, but we might have a concrete value for the particular attr we care about
+  | .set xs              => do
+    let vs ← xs.mapM₁ (fun ⟨x₁, _⟩ => partialEvaluate x₁ req es)
+    match vs.mapM (fun pval => match pval with | .value v => some v | .residual _ => none) with
+    | some vs => ok (.value (Set.make vs))
+    | none    => ok (.residual (PartialExpr.set (vs.map PartialValue.asPartialExpr)))
+  | .record axs          => do
+    let avs ← axs.mapM₂ (fun ⟨(a₁, x₁), _⟩ => partialBindAttr a₁ (partialEvaluate x₁ req es))
+    match avs.mapM (fun (a, pval) => match pval with | .value v => some (a, v) | .residual _ => none) with
+    | some avs => ok (.value (Map.make avs))
+    | none     => ok (.residual (PartialExpr.record (avs.map fun (a, v) => (a, v.asPartialExpr))))
+  | .call xfn xs         => do
+    let vs ← xs.mapM₁ (fun ⟨x₁, _⟩ => partialEvaluate x₁ req es)
+    match vs.mapM (fun pval => match pval with | .value v => some v | .residual _ => none) with
+    | some vs => do
+      let val ← call xfn vs
+      ok (.value val)
+    | none    => ok (.residual (PartialExpr.call xfn (vs.map PartialValue.asPartialExpr)))
+  | .unknown name        => ok (.residual (PartialExpr.unknown name))
