cedar-lean/Cedar/Spec/PartialAuthorizer.lean
@@ -1,0 +1,99 @@
+/-
+ Copyright 2022-2023 Amazon.com, Inc. or its affiliates. All Rights Reserved.
+
+ Licensed under the Apache License, Version 2.0 (the "License");
+ you may not use this file except in compliance with the License.
+ You may obtain a copy of the License at
+
+      https://www.apache.org/licenses/LICENSE-2.0
+
+ Unless required by applicable law or agreed to in writing, software
+ distributed under the License is distributed on an "AS IS" BASIS,
+ WITHOUT WARRANTIES OR CONDITIONS OF ANY KIND, either express or implied.
+ See the License for the specific language governing permissions and
+ limitations under the License.
+-/
+
+import Cedar.Spec.PartialEvaluator
+import Cedar.Spec.PartialResponse
+
+/-! This file defines the Cedar partial authorizer. -/
+
+namespace Cedar.Spec
+
+open Cedar.Data
+open Effect
+
+def knownSatisfied (policy : Policy) (req : PartialRequest) (entities : PartialEntities) : Bool :=
+  partialEvaluate policy.toExpr req entities = .ok (.value true)
+
+def knownUnsatisfied (policy : Policy) (req : PartialRequest) (entities : PartialEntities) : Bool :=
+  partialEvaluate policy.toExpr req entities = .ok (.value false)
+
+def knownSatisfiedWithEffect (effect : Effect) (policy : Policy) (req : PartialRequest) (entities : PartialEntities) : Option PolicyID :=
+  if policy.effect == effect && knownSatisfied policy req entities
+  then some policy.id
+  else none
+
+def knownErroring (policy : Policy) (req : PartialRequest) (entities : PartialEntities) : Bool :=
+  match (partialEvaluate policy.toExpr req entities) with
+  | .ok _ => false
+  | .error _ => true
+
+def knownSatisfiedPolicies (effect : Effect) (policies : Policies) (req : PartialRequest) (entities : PartialEntities) : Set PolicyID :=
+  Set.make (policies.filterMap (knownSatisfiedWithEffect effect · req entities))
+
+/--
+  This function is analogous to `knownSatisfiedWithEffect` in that it returns
+  `Option PolicyID`, but not analogous to `knownSatisfiedWithEffect` in that it does
+  not consider the policy's effect.
+-/
+def knownErroring' (policy : Policy) (req : PartialRequest) (entities : PartialEntities) : Option PolicyID :=
+  if knownErroring policy req entities
+  then some policy.id
+  else none
+
+def knownErroringPolicies (policies : Policies) (req : PartialRequest) (entities : PartialEntities) : Set PolicyID :=
+  Set.make (policies.filterMap (knownErroring' · req entities))
+
+/--
+  If evaluating the policy with these partial inputs results in a residual, return
+  that residual, otherwise None.
+  Returns None for any policies that fully evaluate or that definitely result in
+  an error.
+-/
+def residual (policy : Policy) (req : PartialRequest) (entities : PartialEntities) : Option Residual :=
+  match partialEvaluate policy.toExpr req entities with
+  | .ok (.residual r) => some {
+      id := policy.id,
+      effect := policy.effect,
+      condition := r,
+    }
+  | _ => none
+
+/--
+  Given a set of policies and partial inputs, partial-evaluate and return the
+  set of residual policies.
+  Ignores any policies that fully evaluate or that definitely result in an error.
+-/
+def residualPolicies (policies : Policies) (req : PartialRequest) (entities : PartialEntities) : List Residual :=
+  policies.filterMap (residual · req entities)
+
+def isAuthorizedPartial (req : PartialRequest) (entities : PartialEntities) (policies : Policies) : PartialResponse :=
+  let knownForbids := knownSatisfiedPolicies .forbid policies req entities
+  let knownPermits := knownSatisfiedPolicies .permit policies req entities
+  let residuals := residualPolicies policies req entities
+  let knownErroringPolicies := knownErroringPolicies policies req entities
+  if !knownForbids.isEmpty
+  then .known { decision := .deny, determiningPolicies := knownForbids, erroringPolicies := knownErroringPolicies } -- TODO this is not correct for determiningPolicies
+  else if !residuals.isEmpty
+  then .residual {
+    residuals,
+    determiningPolicies := Set.make (residuals.map Residual.id ++ knownPermits.elts),
+    erroringPolicies := knownErroringPolicies,
+  }
+  else if !knownPermits.isEmpty
+  then .known { decision := .allow, determiningPolicies := knownPermits, erroringPolicies := knownErroringPolicies }
+  else .known { decision := .deny, determiningPolicies := Set.empty, erroringPolicies := knownErroringPolicies }
+
+end Cedar.Spec
