cedar-lean/Cedar/Spec/PartialEntities.lean
@@ -1,0 +1,104 @@
+/-
+ Copyright 2022-2023 Amazon.com, Inc. or its affiliates. All Rights Reserved.
+
+ Licensed under the Apache License, Version 2.0 (the "License");
+ you may not use this file except in compliance with the License.
+ You may obtain a copy of the License at
+
+      https://www.apache.org/licenses/LICENSE-2.0
+
+ Unless required by applicable law or agreed to in writing, software
+ distributed under the License is distributed on an "AS IS" BASIS,
+ WITHOUT WARRANTIES OR CONDITIONS OF ANY KIND, either express or implied.
+ See the License for the specific language governing permissions and
+ limitations under the License.
+-/
+
+import Cedar.Spec.Entities
+import Cedar.Spec.PartialValue
+
+/-!
+This file defines Cedar partial-entities structures.
+-/
+
+namespace Cedar.Spec
+
+open Except
+open Cedar.Data
+
+/--
+Represents the information about one entity.
+
+Currently, this allows attrs to be known-to-exist-but-unknown-value,
+but does not allow attrs to be unknown-whether-they-exist-entirely.
+(the result of `e has attr` is never a residual for an `e` that is known to exist.)
+
+Currently, this does not allow any unknowns about ancestor information.
+All ancestor information must be fully concrete.
+-/
+structure PartialEntityData where
+  attrs : Map Attr PartialValue
+  ancestors : Set EntityUID
+
+def EntityData.asPartialEntityData (d : EntityData) : PartialEntityData :=
+  {
+    attrs := d.attrs.mapOnValues PartialValue.value,
+    ancestors := d.ancestors,
+  }
+
+/--
+Represents the information about all entities.
+
+Currently, this does not allow it to be unknown whether an entity exists.
+Either it exists (and we have a PartialEntityData) or it does not.
+-/
+abbrev PartialEntities := Map EntityUID PartialEntityData
+
+def PartialEntities.ancestors (es : PartialEntities) (uid : EntityUID) : Result (Set EntityUID) := do
+  let d ← es.findOrErr uid .entityDoesNotExist
+  ok d.ancestors
+
+def PartialEntities.ancestorsOrEmpty (es : PartialEntities) (uid : EntityUID) : Set EntityUID :=
+  match es.find? uid with
+  | some d => d.ancestors
+  | none   => Set.empty
+
+def PartialEntities.attrs (es : PartialEntities) (uid : EntityUID) : Result (Map Attr PartialValue) := do
+  let d ← es.findOrErr uid .entityDoesNotExist
+  ok d.attrs
+
+def PartialEntities.attrsOrEmpty (es : PartialEntities) (uid : EntityUID) : Map Attr PartialValue :=
+  match es.find? uid with
+  | some d => d.attrs
+  | none   => Map.empty
+
+deriving instance Repr, DecidableEq, Inhabited for PartialEntityData
+
+def Entities.asPartialEntities (es : Entities) : PartialEntities :=
+  es.mapOnValues EntityData.asPartialEntityData
+
+instance : Coe Entities PartialEntities where
+  coe := Entities.asPartialEntities
+
+/--
+  Given a map of unknown-name to value, substitute all unknowns with the
+  corresponding values, producing a new PartialEntityData.
+  It's fine for some unknowns to not be in `subsmap`, in which case the returned
+  `PartialEntityData` will still contain some unknowns.
+-/
+def PartialEntityData.subst (d : PartialEntityData) (subsmap : Map String PartialValue) : PartialEntityData :=
+  {
+    attrs := d.attrs.mapOnValues (PartialValue.subst · subsmap),
+    ancestors := d.ancestors,
+  }
+
+/--
+  Given a map of unknown-name to value, substitute all unknowns with the
+  corresponding values, producing a new PartialEntities.
+  It's fine for some unknowns to not be in `subsmap`, in which case the returned
+  `PartialEntities` will still contain some unknowns.
+-/
+def PartialEntities.subst (es : PartialEntities) (subsmap : Map String PartialValue) : PartialEntities :=
+  es.mapOnValues (PartialEntityData.subst · subsmap)
+
+end Cedar.Spec
