cedar-lean/Cedar/Spec/PartialExpr.lean
@@ -1,0 +1,178 @@
+/-
+ Copyright 2022-2023 Amazon.com, Inc. or its affiliates. All Rights Reserved.
+
+ Licensed under the Apache License, Version 2.0 (the "License");
+ you may not use this file except in compliance with the License.
+ You may obtain a copy of the License at
+
+      https://www.apache.org/licenses/LICENSE-2.0
+
+ Unless required by applicable law or agreed to in writing, software
+ distributed under the License is distributed on an "AS IS" BASIS,
+ WITHOUT WARRANTIES OR CONDITIONS OF ANY KIND, either express or implied.
+ See the License for the specific language governing permissions and
+ limitations under the License.
+-/
+
+import Cedar.Data
+import Cedar.Spec.Expr
+
+/-! This file defines abstract syntax for Cedar expressions. -/
+
+namespace Cedar.Spec
+
+open Cedar.Data
+
+/--
+  Identical to `Expr` except that it has an `unknown` case, and the recursive
+  elements are also all `PartialExpr` instead of `Expr`
+-/
+inductive PartialExpr where
+  | lit (p : Prim)
+  | var (v : Var)
+  | ite (cond : PartialExpr) (thenExpr : PartialExpr) (elseExpr : PartialExpr)
+  | and (a : PartialExpr) (b : PartialExpr)
+  | or (a : PartialExpr) (b : PartialExpr)
+  | unaryApp (op : UnaryOp) (expr : PartialExpr)
+  | binaryApp (op : BinaryOp) (a : PartialExpr) (b : PartialExpr)
+  | getAttr (expr : PartialExpr) (attr : Attr)
+  | hasAttr (expr : PartialExpr) (attr : Attr)
+  | set (ls : List PartialExpr)
+  | record (map : List (Prod Attr PartialExpr))
+  | call (xfn : ExtFun) (args : List PartialExpr)
+  | unknown (name : String)
+
+deriving instance Repr, Inhabited for PartialExpr
+
+mutual
+
+-- We should be able to get rid of this manual deriviation eventually.
+-- There is work in progress on making these mutual derivations automatic.
+
+def decPartialExpr (x y : PartialExpr) : Decidable (x = y) := by
+  cases x <;> cases y <;>
+  try { apply isFalse ; intro h ; injection h }
+  case lit.lit x₁ y₁ | var.var x₁ y₁ | unknown.unknown x₁ y₁ =>
+    exact match decEq x₁ y₁ with
+    | isTrue h => isTrue (by rw [h])
+    | isFalse _ => isFalse (by intro h; injection h; contradiction)
+  case ite.ite x₁ x₂ x₃ y₁ y₂ y₃ =>
+    exact match decPartialExpr x₁ y₁, decPartialExpr x₂ y₂, decPartialExpr x₃ y₃ with
+    | isTrue h₁, isTrue h₂, isTrue h₃ => isTrue (by rw [h₁, h₂, h₃])
+    | isFalse _, _, _ | _, isFalse _, _ | _, _, isFalse _ => isFalse (by intro h; injection h; contradiction)
+  case and.and x₁ x₂ y₁ y₂ | or.or x₁ x₂ y₁ y₂ =>
+    exact match decPartialExpr x₁ y₁, decPartialExpr x₂ y₂ with
+    | isTrue h₁, isTrue h₂ => isTrue (by rw [h₁, h₂])
+    | isFalse _, _ | _, isFalse _ => isFalse (by intro h; injection h; contradiction)
+  case unaryApp.unaryApp o x₁ o' y₁ =>
+    exact match decEq o o', decPartialExpr x₁ y₁ with
+    | isTrue h₁, isTrue h₂ => isTrue (by rw [h₁, h₂])
+    | isFalse _, _ | _, isFalse _ => isFalse (by intro h; injection h; contradiction)
+  case binaryApp.binaryApp o x₁ x₂ o' y₁ y₂ =>
+    exact match decEq o o', decPartialExpr x₁ y₁, decPartialExpr x₂ y₂ with
+    | isTrue h₁, isTrue h₂, isTrue h₃ => isTrue (by rw [h₁, h₂, h₃])
+    | isFalse _, _, _ | _, isFalse _, _ | _, _, isFalse _ => isFalse (by intro h; injection h; contradiction)
+  case getAttr.getAttr x₁ a y₁ a' | hasAttr.hasAttr x₁ a y₁ a' =>
+    exact match decPartialExpr x₁ y₁, decEq a a' with
+    | isTrue h₁, isTrue h₂ => isTrue (by rw [h₁, h₂])
+    | isFalse _, _ | _, isFalse _ => isFalse (by intro h; injection h; contradiction)
+  case set.set xs ys =>
+    exact match decPartialExprList xs ys with
+    | isTrue h₁ => isTrue (by rw [h₁])
+    | isFalse _ => isFalse (by intro h; injection h; contradiction)
+  case record.record axs ays =>
+    exact match decProdAttrPartialExprList axs ays with
+    | isTrue h₁ => isTrue (by rw [h₁])
+    | isFalse _ => isFalse (by intro h; injection h; contradiction)
+  case call.call f xs f' ys =>
+    exact match decEq f f', decPartialExprList xs ys with
+    | isTrue h₁, isTrue h₂ => isTrue (by rw [h₁, h₂])
+    | isFalse _, _ | _, isFalse _ => isFalse (by intro h; injection h; contradiction)
+
+def decProdAttrPartialExprList (axs ays : List (Prod Attr PartialExpr)) : Decidable (axs = ays) :=
+  match axs, ays with
+  | [], [] => isTrue rfl
+  | _::_, [] | [], _::_ => isFalse (by intro; contradiction)
+  | (a, x)::axs, (a', y)::ays =>
+    match decEq a a', decPartialExpr x y, decProdAttrPartialExprList axs ays with
+    | isTrue h₁, isTrue h₂, isTrue h₃ => isTrue (by rw [h₁, h₂, h₃])
+    | isFalse _, _, _ | _, isFalse _, _ | _, _, isFalse _ =>
+      isFalse (by simp; intros; first | contradiction | assumption)
+
+def decPartialExprList (xs ys : List PartialExpr) : Decidable (xs = ys) :=
+  match xs, ys with
+  | [], [] => isTrue rfl
+  | _::_, [] | [], _::_ => isFalse (by intro; contradiction)
+  | x::xs, y::ys =>
+    match decPartialExpr x y, decPartialExprList xs ys with
+    | isTrue h₁, isTrue h₂ => isTrue (by rw [h₁, h₂])
+    | isFalse _, _ | _, isFalse _ => isFalse (by intro h; injection h; contradiction)
+end
+
+instance : DecidableEq PartialExpr := decPartialExpr
+
+def Expr.asPartialExpr (x : Expr) : PartialExpr :=
+  match x with
+  | .lit p => .lit p
+  | .var v => .var v
+  | .ite x₁ x₂ x₃ => .ite x₁.asPartialExpr x₂.asPartialExpr x₃.asPartialExpr
+  | .and x₁ x₂ => .and x₁.asPartialExpr x₂.asPartialExpr
+  | .or x₁ x₂ => .or x₁.asPartialExpr x₂.asPartialExpr
+  | .unaryApp op x₁ => .unaryApp op x₁.asPartialExpr
+  | .binaryApp op x₁ x₂ => .binaryApp op x₁.asPartialExpr x₂.asPartialExpr
+  | .getAttr x₁ attr => .getAttr x₁.asPartialExpr attr
+  | .hasAttr x₁ attr => .hasAttr x₁.asPartialExpr attr
+  | .set xs => .set (xs.map Expr.asPartialExpr)
+  | .record attrs => .record (attrs.map fun (k, v) => (k, v.asPartialExpr))
+  | .call xfn args => .call xfn (args.map Expr.asPartialExpr)
+decreasing_by sorry
+
+instance : Coe Expr PartialExpr where
+  coe := Expr.asPartialExpr
+
+def PartialExpr.isUnknown (x : PartialExpr) : Bool :=
+  match x with
+  | .unknown _ => true
+  | _ => false
+
+/--
+  Get a list of all the subexpressions of a given expression.
+  Every expression is also a subexpression of itself.
+-/
+def PartialExpr.subexpressions (x : PartialExpr) : List PartialExpr :=
+  match x with
+  | .lit _ => [x]
+  | .var _ => [x]
+  | .ite x₁ x₂ x₃ => [x] ++ x₁.subexpressions ++ x₂.subexpressions ++ x₃.subexpressions
+  | .and x₁ x₂ => [x] ++ x₁.subexpressions ++ x₂.subexpressions
+  | .or x₁ x₂ => [x] ++ x₁.subexpressions ++ x₂.subexpressions
+  | .unaryApp _ x₁ => [x] ++ x₁.subexpressions
+  | .binaryApp _ x₁ x₂ => [x] ++ x₁.subexpressions ++ x₂.subexpressions
+  | .getAttr x₁ _ => [x] ++ x₁.subexpressions
+  | .hasAttr x₁ _ => [x] ++ x₁.subexpressions
+  | .set xs => [x] ++ List.join (xs.map PartialExpr.subexpressions)
+  | .record pairs => [x] ++ List.join (pairs.map fun (_, x₁) => x₁.subexpressions)
+  | .call _ xs => [x] ++ List.join (xs.map PartialExpr.subexpressions)
+  | .unknown _ => [x]
+decreasing_by sorry
+
+/--
+  Does a given PartialExpr contain an Unknown, perhaps recursively
+-/
+def PartialExpr.containsUnknown (x : PartialExpr) : Bool :=
+  x.subexpressions.any PartialExpr.isUnknown
+
+/--
+  Is a given PartialExpr fully concrete (no Unknowns even recursively)
+-/
+def PartialExpr.fullyConcrete (x : PartialExpr) : Bool :=
+  ¬ x.containsUnknown
+
+/--
+  any expression is a subexpression of itself
+-/
+theorem PartialExpr.subexpression_refl {x : PartialExpr} :
+  x ∈ x.subexpressions
+:= by
+  unfold PartialExpr.subexpressions
+  cases x <;> simp
