cedar-lean/Cedar/Spec/PartialResponse.lean
@@ -1,0 +1,51 @@
+/-
+ Copyright 2022-2023 Amazon.com, Inc. or its affiliates. All Rights Reserved.
+
+ Licensed under the Apache License, Version 2.0 (the "License");
+ you may not use this file except in compliance with the License.
+ You may obtain a copy of the License at
+
+      https://www.apache.org/licenses/LICENSE-2.0
+
+ Unless required by applicable law or agreed to in writing, software
+ distributed under the License is distributed on an "AS IS" BASIS,
+ WITHOUT WARRANTIES OR CONDITIONS OF ANY KIND, either express or implied.
+ See the License for the specific language governing permissions and
+ limitations under the License.
+-/
+
+import Cedar.Spec.PartialExpr
+import Cedar.Spec.Policy
+import Cedar.Spec.Response
+
+/-!
+This file defines Cedar partial responses.
+-/
+
+namespace Cedar.Spec
+
+open Cedar.Data
+
+----- Definitions -----
+
+structure Residual where
+  id : PolicyID
+  effect : Effect
+  condition : PartialExpr
+
+structure ResidualResponse where
+  residuals : List Residual
+  determiningPolicies : Set PolicyID -- all policies that could possibly be determining, for any assignment of the unknowns
+  erroringPolicies : Set PolicyID -- all policies that could possibly be erroring, for any assignment of the unknowns
+
+inductive PartialResponse where
+  | known (resp : Response)
+  | residual (resp : ResidualResponse)
+
+----- Derivations -----
+
+deriving instance Repr, DecidableEq for Residual
+deriving instance Repr, DecidableEq for ResidualResponse
+deriving instance Repr, DecidableEq for PartialResponse
+
+end Cedar.Spec
