cedar-lean/Cedar/Spec/PartialValue.lean
@@ -1,0 +1,113 @@
+/-
+ Copyright 2022-2023 Amazon.com, Inc. or its affiliates. All Rights Reserved.
+
+ Licensed under the Apache License, Version 2.0 (the "License");
+ you may not use this file except in compliance with the License.
+ You may obtain a copy of the License at
+
+      https://www.apache.org/licenses/LICENSE-2.0
+
+ Unless required by applicable law or agreed to in writing, software
+ distributed under the License is distributed on an "AS IS" BASIS,
+ WITHOUT WARRANTIES OR CONDITIONS OF ANY KIND, either express or implied.
+ See the License for the specific language governing permissions and
+ limitations under the License.
+-/
+
+import Cedar.Data.Map
+import Cedar.Spec.Ext.IPAddr
+import Cedar.Spec.Value
+import Cedar.Spec.PartialExpr
+
+/-!
+This file defines Cedar partial values.
+-/
+
+namespace Cedar.Spec
+
+open Cedar.Data
+
+inductive PartialValue where
+  | value (v : Value)
+  | residual (r : PartialExpr)
+
+deriving instance Repr, DecidableEq, Inhabited for PartialValue
+
+def Value.asPartialExpr (v : Value) : PartialExpr :=
+  match v with
+  | .prim p => PartialExpr.lit p
+  | .set s => PartialExpr.set (s.elts.map Value.asPartialExpr)
+  | .record m => PartialExpr.record (m.kvs.map fun (k, v)=> (k, v.asPartialExpr))
+  | .ext (.decimal d) => PartialExpr.call ExtFun.decimal [PartialExpr.lit (.string d.unParse)]
+  | .ext (.ipaddr ip) => PartialExpr.call ExtFun.ip [PartialExpr.lit (.string (Cedar.Spec.Ext.IPAddr.unParse ip))]
+decreasing_by sorry
+
+def PartialValue.asPartialExpr (v : PartialValue) : PartialExpr :=
+  match v with
+  | .value v    => Value.asPartialExpr v
+  | .residual r => r
+
+/--
+  Given a map of unknown-name to value, substitute all unknowns with the
+  corresponding values, producing a new PartialExpr.
+  It's fine for some unknowns to not be in `subsmap`, in which case the returned
+  `PartialExpr` will still contain some unknowns.
+-/
+-- NB: this function can't live in PartialExpr.lean because it needs PartialValue, and
+-- PartialExpr.lean can't import PartialValue, cyclic dependency
+def PartialExpr.subst (x : PartialExpr) (subsmap : Map String PartialValue) : PartialExpr :=
+  match x with
+  | .lit _ => x -- no unknowns, nothing to substitute
+  | .var _ => x -- no unknowns, nothing to substitute
+  | .ite x₁ x₂ x₃ =>
+    let x₁' := x₁.subst subsmap
+    let x₂' := x₂.subst subsmap
+    let x₃' := x₃.subst subsmap
+    .ite x₁' x₂' x₃'
+  | .and x₁ x₂ =>
+    let x₁' := x₁.subst subsmap
+    let x₂' := x₂.subst subsmap
+    .and x₁' x₂'
+  | .or x₁ x₂ =>
+    let x₁' := x₁.subst subsmap
+    let x₂' := x₂.subst subsmap
+    .or x₁' x₂'
+  | .unaryApp op x₁ =>
+    let x₁' := x₁.subst subsmap
+    .unaryApp op x₁
+  | .binaryApp op x₁ x₂ =>
+    let x₁' := x₁.subst subsmap
+    let x₂' := x₂.subst subsmap
+    .binaryApp op x₁' x₂'
+  | .getAttr x₁ attr =>
+    let x₁' := x₁.subst subsmap
+    .getAttr x₁' attr
+  | .hasAttr x₁ attr =>
+    let x₁' := x₁.subst subsmap
+    .hasAttr x₁' attr
+  | .set xs =>
+    let xs' := xs.map (PartialExpr.subst · subsmap)
+    .set xs'
+  | .record pairs =>
+    let pairs' := pairs.map fun (k, v) => (k, v.subst subsmap)
+    .record pairs'
+  | .call xfn xs =>
+    let xs' := xs.map (PartialExpr.subst · subsmap)
+    .call xfn xs'
+  | unknown name => match subsmap.find? name with
+    | some val => val.asPartialExpr
+    | none => x -- no substitution available, return `x` unchanged
+decreasing_by sorry
+
+/--
+  Given a map of unknown-name to value, substitute all unknowns with the
+  corresponding values, producing a new PartialValue.
+  It's fine for some unknowns to not be in `subsmap`, in which case the returned
+  `PartialValue` will still contain some unknowns.
+-/
+def PartialValue.subst (v : PartialValue) (subsmap : Map String PartialValue) : PartialValue :=
+  match v with
+  | .residual r => .residual (r.subst subsmap)
+  | .value v    => .value v -- doesn't contain unknowns, nothing to substitute
+
+end Cedar.Spec
