cedar-lean/Cedar/Thm/PartialAuthorization.lean
@@ -1,0 +1,162 @@
+/-
+ Copyright 2022-2023 Amazon.com, Inc. or its affiliates. All Rights Reserved.
+
+ Licensed under the Apache License, Version 2.0 (the "License");
+ you may not use this file except in compliance with the License.
+ You may obtain a copy of the License at
+
+      https://www.apache.org/licenses/LICENSE-2.0
+
+ Unless required by applicable law or agreed to in writing, software
+ distributed under the License is distributed on an "AS IS" BASIS,
+ WITHOUT WARRANTIES OR CONDITIONS OF ANY KIND, either express or implied.
+ See the License for the specific language governing permissions and
+ limitations under the License.
+-/
+
+import Cedar.Spec.Value
+import Cedar.Spec.PartialAuthorizer
+import Cedar.Spec.PartialResponse
+import Cedar.Thm.PartialEval
+import Cedar.Thm.PartialEval.And
+import Cedar.Thm.Utils
+
+/-! This file contains theorems about Cedar's partial evaluator. -/
+
+namespace Cedar.Thm
+
+open Cedar.Data
+open Cedar.Spec
+open Except
+
+/--
+  just a sanity-check theorem about implementation details of isAuthorizedPartial:
+  for any given set of partial inputs, every policy is either knownSatisfied,
+  knownUnsatisfied, knownErroring, or residual
+-/
+theorem policy_cases {policy : Policy} {req : PartialRequest} {entities : PartialEntities} :
+  knownSatisfied policy req entities ∨
+  knownUnsatisfied policy req entities ∨
+  knownErroring policy req entities ∨
+  (residual policy req entities).isSome
+:= by
+  unfold knownSatisfied knownUnsatisfied knownErroring residual
+  cases h₁ : (partialEvaluate policy.toExpr req entities) <;> simp [h₁]
+  case ok pval =>
+    unfold Policy.toExpr at h₁
+    have h₂ := @partial_exprand_produces_bool_residual_or_error policy.principalScope.toExpr (Expr.and policy.actionScope.toExpr (Expr.and policy.resourceScope.toExpr policy.condition)) req entities
+    simp [h₁] at h₂
+    cases pval <;> try cases h₂
+    case residual r => simp
+    case value v =>
+      cases v <;> try cases h₂
+      case prim p =>
+        cases p <;> try cases h₂
+        case bool.intro b =>
+          cases b <;> simp
+
+/--
+  helper lemma:
+  residualPolicies produces the empty set when applied to concrete inputs
+-/
+theorem residualPolicies_empty_on_concrete {policies : Policies} {req : Request} {entities : Entities} :
+  residualPolicies policies req entities = []
+:= by
+  unfold residualPolicies residual
+  simp [partial_eval_on_concrete_eqv_concrete_eval, Except.map]
+  simp [List.filterMap_empty_iff_f_returns_none]
+  intro p _
+  split <;> simp
+  rename_i r h₂
+  generalize (evaluate p.toExpr req entities) = res at h₂
+  split at h₂ <;> simp at h₂
+
+/--
+  helper lemma:
+  knownSatisfied is the same as satisfied if all inputs are concrete
+-/
+theorem knownSatisfied_eqv_satisfied_on_concrete {policy : Policy} {req : Request} {entities : Entities} :
+  knownSatisfied policy req entities = satisfied policy req entities
+:= by
+  unfold knownSatisfied satisfied
+  simp [partial_eval_on_concrete_eqv_concrete_eval, Except.map]
+  split <;> rename_i h <;> simp [h]
+
+/--
+  helper lemma:
+  knownSatisfiedPolicies is the same as satisfiedPolicies if all inputs are concrete
+-/
+theorem knownSatisfiedPolicies_eqv_satisfiedPolicies_on_concrete {effect : Effect} {policies : Policies} {req : Request} {entities : Entities} :
+  knownSatisfiedPolicies effect policies req entities = satisfiedPolicies effect policies req entities
+:= by
+  unfold knownSatisfiedPolicies satisfiedPolicies
+  rw [Set.make_make_eqv]
+  unfold knownSatisfiedWithEffect satisfiedWithEffect
+  simp [knownSatisfied_eqv_satisfied_on_concrete, List.Equiv]
+
+/--
+  helper lemma:
+  knownErroring is the same as hasError if all inputs are concrete
+-/
+theorem knownErroring_eqv_hasError_on_concrete {policy : Policy} {req : Request} {entities : Entities} :
+  knownErroring policy req entities = hasError policy req entities
+:= by
+  unfold knownErroring hasError
+  simp [partial_eval_on_concrete_eqv_concrete_eval, Except.map]
+  split <;> rename_i h₁ <;> split at h₁
+  case _ => simp at h₁
+  case _ => rename_i h₂ ; simp [h₂]
+  case _ => rename_i h₂ ; simp [h₂]
+  case _ => simp at h₁
+
+/--
+  helper lemma:
+  knownErroringPolicies is the same as errorPolicies if all inputs are concrete
+-/
+theorem knownErroringPolicies_eqv_errorPolicies_on_concrete {policies : Policies} {req : Request} {entities : Entities} :
+  knownErroringPolicies policies req entities = errorPolicies policies req entities
+:= by
+  unfold knownErroringPolicies errorPolicies
+  rw [Set.make_make_eqv]
+  unfold knownErroring' errored
+  simp [knownErroring_eqv_hasError_on_concrete, List.Equiv]
+
+/--
+  Partial-authorizing with concrete inputs gives the same concrete outputs as
+  concrete-authorizing with those inputs.
+
+  Corollary to this: partial-authorizing with concrete inputs never gives a
+  residual response.
+-/
+theorem partial_authz_eqv_authz_on_concrete {policies : Policies} {req : Request} {entities : Entities} :
+  isAuthorizedPartial req entities policies = .known (isAuthorized req entities policies)
+:= by
+  unfold isAuthorizedPartial isAuthorized
+  simp [knownSatisfiedPolicies_eqv_satisfiedPolicies_on_concrete, knownErroringPolicies_eqv_errorPolicies_on_concrete, residualPolicies_empty_on_concrete, Set.isEmpty]
+  split <;> rename_i h₁ <;> simp [h₁]
+  split <;> simp
+
+/--
+  helper lemma: if partial authorization returns .known, then residualPolicies
+  is the empty set
+-/
+theorem partial_authz_known_then_residualPolicies_empty {policies : Policies} {req : PartialRequest} {entities : PartialEntities} {resp : Response} :
+  isAuthorizedPartial req entities policies = .known resp →
+  residualPolicies policies req entities = []
+:= by
+  sorry
+
+/--
+  If partial authorization returns .known, then that result is identical
+  (including diagnostics) to the result you'd get with any (valid) substitution
+  for the unknowns.
+-/
+theorem partial_authz_known_then_unknown_agnostic {policies : Policies} {req req': PartialRequest} {entities : PartialEntities} {subsmap : Map String PartialValue} :
+  req.subst subsmap = some req' →
+  isAuthorizedPartial req entities policies = .known resp →
+  isAuthorizedPartial req' (entities.subst subsmap) policies = .known resp
+:= by
+  intro h₁ h₂
+  have h₃ := partial_authz_known_then_residualPolicies_empty h₂
+  simp [isAuthorizedPartial]
+  sorry
