cedar-lean/Cedar/Thm/PartialEval.lean
@@ -1,0 +1,93 @@
+/-
+ Copyright 2022-2023 Amazon.com, Inc. or its affiliates. All Rights Reserved.
+
+ Licensed under the Apache License, Version 2.0 (the "License");
+ you may not use this file except in compliance with the License.
+ You may obtain a copy of the License at
+
+      https://www.apache.org/licenses/LICENSE-2.0
+
+ Unless required by applicable law or agreed to in writing, software
+ distributed under the License is distributed on an "AS IS" BASIS,
+ WITHOUT WARRANTIES OR CONDITIONS OF ANY KIND, either express or implied.
+ See the License for the specific language governing permissions and
+ limitations under the License.
+-/
+
+import Cedar.Spec.Evaluator
+import Cedar.Spec.PartialEvaluator
+import Cedar.Thm.PartialEval.And
+import Cedar.Thm.PartialEval.Basic
+import Cedar.Thm.Utils
+
+/-! This file contains theorems about Cedar's partial evaluator. -/
+
+namespace Cedar.Thm
+
+open Cedar.Data
+open Cedar.Spec
+open Except
+
+/--
+  Partial evaluation with concrete inputs gives the same output as
+  concrete evaluation with those inputs
+-/
+theorem partial_eval_on_concrete_eqv_concrete_eval {expr : Expr} {request : Request} {entities : Entities} :
+  partialEvaluate expr request entities = (evaluate expr request entities).map PartialValue.value
+:= by
+  unfold partialEvaluate evaluate Except.map
+  cases expr <;> simp [Expr.asPartialExpr]
+  case var v =>
+    cases v <;> simp [Request.asPartialRequest]
+    case context =>
+      split <;> simp
+      case h_1 kvs h =>
+        -- induction on kvs?
+        sorry
+      case h_2 =>
+        sorry
+  case and x₁ x₂ =>
+    -- need some kind of inductive argument where we can assume the theorem on the subexpressions
+    sorry
+  case or x₁ x₂ =>
+    sorry
+  case ite x₁ x₂ x₃ =>
+    sorry
+  all_goals {
+    sorry
+  }
+
+/--
+  If partial evaluation returns a residual, then that residual expression
+  contains an unknown
+-/
+theorem residuals_contain_unknowns {expr : PartialExpr} {request : PartialRequest} {entities : PartialEntities} {r : PartialExpr} :
+  partialEvaluate expr request entities = ok (.residual r) →
+  r.containsUnknown
+:= by
+  unfold partialEvaluate PartialExpr.containsUnknown
+  cases expr <;> simp <;> intro h₁
+  case var v =>
+    cases v <;> simp at h₁
+    case principal =>
+      cases h₂ : request.principal <;> simp [h₂] at h₁
+      case unknown name =>
+        subst h₁
+        simp [PartialExpr.subexpressions, PartialExpr.isUnknown]
+    case action =>
+      cases h₂ : request.action <;> simp [h₂] at h₁
+      case unknown name =>
+        subst h₁
+        simp [PartialExpr.subexpressions, PartialExpr.isUnknown]
+    case resource =>
+      cases h₂ : request.resource <;> simp [h₂] at h₁
+      case unknown name =>
+        subst h₁
+        simp [PartialExpr.subexpressions, PartialExpr.isUnknown]
+    case context =>
+      sorry
+  case and x₁ x₂ =>
+    sorry
+  all_goals {
+    sorry
+  }
