cedar-lean/Cedar/Thm/PartialEval/And.lean
@@ -1,0 +1,172 @@
+/-
+ Copyright 2022-2023 Amazon.com, Inc. or its affiliates. All Rights Reserved.
+
+ Licensed under the Apache License, Version 2.0 (the "License");
+ you may not use this file except in compliance with the License.
+ You may obtain a copy of the License at
+
+      https://www.apache.org/licenses/LICENSE-2.0
+
+ Unless required by applicable law or agreed to in writing, software
+ distributed under the License is distributed on an "AS IS" BASIS,
+ WITHOUT WARRANTIES OR CONDITIONS OF ANY KIND, either express or implied.
+ See the License for the specific language governing permissions and
+ limitations under the License.
+-/
+
+import Cedar.Spec.PartialEvaluator
+import Cedar.Thm.PartialEval.Basic
+
+namespace Cedar.Thm
+
+open Cedar.Spec
+open Except
+
+/--
+  helper lemma: any subexpression of x₁ is a subexpression of (x₁ && x₂)
+-/
+theorem and_lhs_subexpression {x₁ x₂ x : PartialExpr}
+  (h₁ : x ∈ x₁.subexpressions) :
+  x ∈ (PartialExpr.and x₁ x₂).subexpressions
+:= by
+  unfold PartialExpr.subexpressions
+  simp [List.append_eq_append]
+  right ; left ; assumption
+
+/--
+  helper lemma: if LHS of a `PartialExpr.and` contains an unknown, the whole expression does
+-/
+theorem and_lhs_unknown {x₁ x₂ : PartialExpr}
+  (h₁ : x₁.containsUnknown) :
+  (PartialExpr.and x₁ x₂).containsUnknown
+:= by
+  unfold PartialExpr.containsUnknown at *
+  rw [List.any_eq_true] at *
+  replace ⟨subx, h₁⟩ := h₁
+  exists subx
+  constructor
+  case left => apply and_lhs_subexpression h₁.left
+  case right => exact h₁.right
+
+/--
+  Inductive argument for `ResidualsContainUnknowns` for `PartialExpr.and`
+-/
+theorem and_residuals_contain_unknowns {x₁ x₂ : PartialExpr}
+  (ih₁ : ResidualsContainUnknowns x₁)
+  (ih₂ : ResidualsContainUnknowns x₂) :
+  ResidualsContainUnknowns (PartialExpr.and x₁ x₂)
+:= by
+  unfold ResidualsContainUnknowns at *
+  intro req es r
+  specialize @ih₁ req es
+  specialize @ih₂ req es
+  unfold partialEvaluate
+  cases h₁ : (partialEvaluate x₁ req es) <;> simp <;> intro h₂
+  case error e => cases h₂
+  case ok pval₁ =>
+    cases pval₁
+    case residual r₁ =>
+      -- partial evaluating the LHS produced a residual
+      specialize ih₁ h₁
+      cases h₂
+      apply and_lhs_unknown
+      assumption
+    case value v₁ =>
+      -- partial evaluating the LHS produced a value v₁
+      cases v₁
+      case set | record | ext => cases h₂
+      case prim p₁ =>
+        cases p₁
+        case int | string | entityUID => cases h₂
+        case bool b₁ =>
+          unfold Value.asBool at h₂
+          cases b₁
+          case false => cases h₂
+          case true =>
+            -- partial evaluating the LHS produced ok-true
+            cases h₃ : (partialEvaluate x₂ req es) <;> simp [h₃] at h₂
+            case error e => cases h₂
+            case ok pval₂ =>
+              cases pval₂
+              case residual r₂ =>
+                -- partial evaluating the RHS produced a residual
+                specialize ih₂ h₃
+                cases h₂
+                assumption
+              case value v₂ =>
+                -- partial evaluating the RHS produced a value v₂
+                cases v₂
+                case set | record | ext => cases h₂
+                case prim p₂ => cases p₂ <;> cases h₂
+
+/--
+  Partial-evaluating a `PartialExpr.and` expression produces either .ok bool, a residual,
+  or an error
+-/
+theorem partialexprand_produces_bool_residual_or_error {e₁ e₂ : PartialExpr} {request : PartialRequest} {entities : PartialEntities} :
+  match (partialEvaluate (PartialExpr.and e₁ e₂) request entities) with
+  | .ok (.value (.prim (.bool _))) => true
+  | .ok (.residual _) => true
+  | .error _ => true
+  | _ => false
+:= by
+  cases h : partialEvaluate (PartialExpr.and e₁ e₂) request entities <;> simp
+  case ok val =>
+    cases val <;> simp [partialEvaluate] at h <;>
+    generalize (partialEvaluate e₁ request entities) = res₁ at h <;>
+    generalize (partialEvaluate e₂ request entities) = res₂ at h
+    case residual r => simp
+    case value v =>
+      simp [Value.asBool] at h
+      cases res₁ <;> cases res₂ <;> try cases h
+      case ok.error pval₁ err₂ =>
+        cases pval₁ <;> try cases h
+        case value v₁ =>
+          cases v₁ <;> try cases h
+          case prim p₁ =>
+            cases p₁ <;> try cases h
+            case bool b =>
+              cases b <;> cases h
+              split <;> trivial
+      case ok.ok pval₁ pval₂ =>
+        cases pval₁ <;> cases pval₂ <;> try cases h
+        case value.value v₁ v₂ =>
+          cases v₁ <;> cases v₂ <;> try cases h
+          case prim.prim p₁ p₂ =>
+            cases p₁ <;> cases p₂ <;> try cases h
+            case bool.bool b₁ b₂ =>
+              cases b₁ <;> cases b₂ <;> cases h
+              all_goals {
+                split <;> trivial
+              }
+            case bool.int b₁ _ | bool.string b₁ _ | bool.entityUID b₁ _ =>
+              cases b₁ <;> cases h
+              split <;> trivial
+          case prim.set p₁ _ | prim.record p₁ _ | prim.ext p₁ _ =>
+            cases p₁ <;> try cases h
+            case bool b₁ =>
+              cases b₁ <;> cases h
+              split <;> trivial
+        case value.residual v₁ r₂ =>
+          cases v₁ <;> try cases h
+          case prim p₁ =>
+            cases p₁ <;> try cases h
+            case bool b₁ =>
+              cases b₁ <;> cases h
+              split <;> trivial
+
+/--
+  Corollary to the above: Partial-evaluating an `Expr.and` expression
+  produces either .ok bool, a residual, or an error
+-/
+theorem partial_exprand_produces_bool_residual_or_error {e₁ e₂ : Expr} {request : PartialRequest} {entities : PartialEntities} :
+  match (partialEvaluate (Expr.and e₁ e₂) request entities) with
+  | .ok (.value (.prim (.bool _))) => true
+  | .ok (.residual _) => true
+  | .error _ => true
+  | _ => false
+:= by
+  unfold Expr.asPartialExpr
+  exact @partialexprand_produces_bool_residual_or_error e₁.asPartialExpr e₂.asPartialExpr request entities
+
+end Cedar.Thm
