cedar-lean/Cedar/Thm/Utils.lean
@@ -1,0 +1,83 @@
+/-
+ Copyright 2022-2023 Amazon.com, Inc. or its affiliates. All Rights Reserved.
+
+ Licensed under the Apache License, Version 2.0 (the "License");
+ you may not use this file except in compliance with the License.
+ You may obtain a copy of the License at
+
+      https://www.apache.org/licenses/LICENSE-2.0
+
+ Unless required by applicable law or agreed to in writing, software
+ distributed under the License is distributed on an "AS IS" BASIS,
+ WITHOUT WARRANTIES OR CONDITIONS OF ANY KIND, either express or implied.
+ See the License for the specific language governing permissions and
+ limitations under the License.
+-/
+
+import Cedar.Data.List
+import Cedar.Spec
+
+/-!
+This file contains useful lemmas about Std and List functions.
+-/
+
+namespace Cedar.Thm
+
+open Cedar.Data
+
+/--
+  A generic lemma that relates List.mapM to List.map. Not in Std AFAICT.
+-/
+theorem if_f_produces_pure_then_mapM_f_is_pure_map {α β} [Monad m] [LawfulMonad m] {f : α → β} {list : List α} :
+  list.mapM ((fun a => pure (f a)) : α → m β) = pure (list.map f)
+:= by
+  induction list
+  case nil => simp
+  case cons x xs h => simp [h]
+
+/--
+  A generic lemma about composing List.mapM with List.map. Not in Std AFAICT.
+-/
+theorem mapM_over_map {α β γ} [Monad m] [LawfulMonad m] {f : α → β} {g : β → m γ} {list : List α} :
+  List.mapM g (list.map f) = list.mapM fun x => g (f x)
+:= by
+  induction list
+  case nil => simp
+  case cons x xs h => simp [h]
+
+/--
+  A generic lemma about the behavior of List.mapM in the Option monad
+-/
+theorem mapM_some_iff_f_some_on_all_elements {f : α → Option β} {list : List α} :
+  Option.isSome (list.mapM f) ↔ ∀ x ∈ list, Option.isSome (f x)
+:= by
+  rw [←List.mapM'_eq_mapM]
+  constructor
+  case mp =>
+    induction list
+    case nil => simp
+    case cons x xs h_ind =>
+      simp [List.mapM'_cons]
+      intro h₁
+      unfold List.mapM' at h₁
+      constructor
+      case left =>
+        cases h₂ : (f x) <;> simp [h₂] at h₁
+        simp
+      case right =>
+        intro a
+        apply h_ind
+        rw [Option.isSome_iff_exists] at h₁
+        replace ⟨list₁, h₁⟩ := h₁
+        cases h₂ : (f x) <;> simp [h₂] at h₁
+        replace ⟨list₂, ⟨h₁, h₂⟩⟩ := h₁
+        simp [Option.bind] at h₁
+        sorry
+  case mpr =>
+    intro h
+    induction list
+    case nil => simp [List.mapM']
+    case cons y ys h_ind =>
+      have h₂ := h y ; simp at h₂
+      rw [List.mapM'_cons]
+      sorry
